Quote sort families

src/reify.mli
@@ -11,18 +11,18 @@ module type Quoter = sig
   type quoted_decl
   type quoted_program
   type quoted_proj
-
+  type quoted_sort_family
   open Names
 
   val quote_ident : Id.t -> quoted_ident
   val quote_name : Name.t -> quoted_name
   val quote_int : int -> quoted_int
   val quote_sort : Sorts.t -> quoted_sort
+  val quote_sort_family : Sorts.family -> quoted_sort_family
   val quote_cast_kind : Constr.cast_kind -> quoted_cast_kind
   val quote_kn : kernel_name -> quoted_kernel_name
   val quote_inductive : quoted_kernel_name * quoted_int -> quoted_inductive
   val quote_proj : quoted_inductive -> quoted_int -> quoted_int -> quoted_proj
-
   val mkName : quoted_ident -> quoted_name
   val mkAnon : quoted_name
 
@@ -48,7 +48,7 @@ module type Quoter = sig
     
 
   val mkMutualInductive : quoted_kernel_name -> quoted_int (* params *) ->
-                          (quoted_ident * t (* ind type *) *
+                          (quoted_ident * t (* ind type *) * quoted_sort_family list *
                              (quoted_ident * t (* constr type *) * quoted_int) list *
                                (quoted_ident * t) list (* projections *)) list ->
                           quoted_decl
